Chapter 19, Program Equivalence

Equiv.v
@@ -38,3 +38,538 @@ Theorem skip_left :
 Qed.
 
 
+Theorem skip_right:
+  forall c,
+    cequiv (c;;SKIP)
+           c.
+  unfold cequiv. split.
+  intros. inversion H. inversion H5. rewrite H8 in H2. auto.
+  intros. eapply E_Seq. apply H. apply E_Skip.
+Qed.
+
+
+Theorem IFB_true_simple :
+  forall c1 c2,
+    cequiv (IFB BTrue THEN c1 ELSE c2 FI)
+           c1.
+  unfold cequiv. split.
+  intros. inversion H; auto. simpl in H5. discriminate.
+  intros. apply E_IfTrue. auto. apply H.
+Qed.
+
+
+Theorem IFB_true :
+  forall b c1 c2,
+    bequiv b BTrue ->
+    cequiv (IFB b THEN c1 ELSE c2 FI)
+           c1.
+
+  split. intros.
+  inversion H0; auto. unfold bequiv in H. pose (H st). rewrite H6 in e. simpl in e. discriminate.
+  intros. apply E_IfTrue. pose (H st). simpl in e; auto.
+  auto.
+Qed.
+
+Theorem swap_if_branches:
+  forall b e1 e2,
+    cequiv (IFB b THEN e1 ELSE e2 FI)
+           (IFB BNot b THEN e2 ELSE e1 FI).
+  unfold cequiv.
+  intros until st.
+  destruct (beval st b) eqn: b1.
+  split. intros. inversion H. apply E_IfFalse. simpl. rewrite H5. auto. auto.
+  apply E_IfTrue. simpl. rewrite H5. auto. auto.
+  intros. inversion H. simpl in H5. rewrite b1 in H5. simpl in H5. discriminate.
+  apply E_IfTrue. auto. auto.
+  split. intros. apply E_IfTrue. simpl; rewrite b1; auto. inversion H. rewrite b1 in H5; discriminate.
+  auto.
+  intros. apply E_IfFalse. auto. inversion H; auto. simpl in H5; rewrite b1 in H5; simpl in H5; discriminate.
+Qed.
+
+
+Theorem WHILE_false :
+  forall b c,
+    bequiv b BFalse ->
+    cequiv (WHILE b DO c END)
+           SKIP.
+
+  intros. split. intros. pose (H st). simpl in e. inversion H0. rewrite e in H3; discriminate.
+  apply E_Skip.
+  intros. inversion H0. apply E_WhileEnd. pose (H st). simpl in e; subst st'; auto.
+Qed.
+
+
+Lemma WHILE_true_nonterm :
+  forall b c st st',
+    bequiv b BTrue ->
+    ~( (WHILE b DO c END) / st \\ st').
+  unfold not. intros. remember (WHILE b DO c END) as h. generalize Heqh.
+  elim H0; try (simpl; intros; discriminate).
+  intros. auto.
+  intros. inversion Heqh0; subst b0.
+  pose (H st0). simpl in e. rewrite e in H1. discriminate.
+Qed.
+
+Theorem WHILE_true :
+  forall b c,
+    bequiv b BTrue ->
+    cequiv (WHILE b DO c END)
+           (WHILE BTrue DO SKIP END).
+  split. intros. pose (WHILE_true_nonterm b c st st'). elim (n H H0).
+  intros. pose (WHILE_true_nonterm BTrue SKIP st st'). unfold bequiv in n.
+  assert (False). apply n. intros; auto. auto. elim H1.
+Qed.
+
+Theorem seq_assoc :
+  forall c1 c2 c3,
+    cequiv ((c1 ;; c2) ;; c3)
+           (c1 ;; (c2 ;; c3)).
+
+  split. intros. inversion H. inversion H2. eapply E_Seq. apply H8. eapply E_Seq. apply H11. auto.
+  intros. inversion H. inversion H5. eapply E_Seq. eapply E_Seq. apply H2. apply H8. apply H11.
+Qed.
+
+Theorem identity_assignment :
+  forall (X:id),
+    cequiv (X ::= AId X)
+           SKIP.
+
+  split. intros. inversion H.
+  assert (st = t_update st X n).
+  apply functional_extensionality.
+  intro. unfold t_update.
+  case (eq_id_dec X x0). intros. simpl in H4. subst x0. auto.
+  auto. pattern st at 1. rewrite H5. apply E_Skip.
+  intros. inversion H.
+  assert (st' = t_update st' X (aeval st' (AId X))).
+  apply functional_extensionality.
+  intro; unfold t_update.
+  case (eq_id_dec X x). simpl. intros; subst x; auto.
+  auto.
+  pattern st' at 2. rewrite H0. eapply E_Ass. auto.
+Qed.
+
+
+
+
+Theorem symm_cequiv:
+  forall a b,
+    cequiv a b <-> cequiv b a.
+  unfold cequiv.
+  intros. split; intros. split; apply (H st st').
+  split; apply (H st st').
+Qed.
+
+Theorem assign_aequiv:
+  forall X e,
+    aequiv (AId X) e ->
+    cequiv SKIP (X ::= e).
+  intros. split; intros.
+  pose (identity_assignment X).
+  unfold cequiv in c. pose (c st st'). destruct i.
+  pose (H2 H0). inversion c0. pose (H st). rewrite e0 in H7. rewrite <- H7.
+  apply E_Ass. auto.
+  apply (identity_assignment X). pose (H st).
+  inversion H0. apply E_Ass. subst n; auto.
+Qed.
+
+Lemma refl_aequiv :
+  forall a,
+    aequiv a a.
+  split.
+Qed.
+
+
+Lemma sym_aequiv:
+  forall a1 a2,
+    aequiv a1 a2 <-> aequiv a2 a1.
+  split; intros;unfold aequiv; intros st; pose (H st); auto.
+Qed.
+
+Lemma trans_aequiv:
+  forall a1 a2 a3,
+    aequiv a1 a2 ->
+    aequiv a2 a3 ->
+    aequiv a1 a3.
+  intros. unfold aequiv. intro. pose (H st); pose (H0 st). rewrite e; rewrite e0; auto.
+Qed.
+
+
+Lemma refl_bequiv:
+  forall b,
+    bequiv b b.
+  split.
+Qed.
+
+Lemma symm_bequiv:
+  forall b1 b2,
+    bequiv b1 b2 -> bequiv b2 b2.
+  unfold bequiv. intros. symmetry in H. auto.
+Qed.
+
+
+Lemma tran_bequiv:
+  forall b1 b2 b3,
+    bequiv b1 b2 ->
+    bequiv b2 b3 ->
+    bequiv b1 b3.
+  unfold bequiv.
+  intros.
+  rewrite H; rewrite H0; auto.
+Qed.
+
+
+Lemma refl_cequiv:
+  forall c,
+    cequiv c c.
+  split; auto.
+Qed.
+
+
+Lemma trans_cequiv :
+  forall c1 c2 c3,
+    cequiv c1 c2 ->
+    cequiv c2 c3 ->
+    cequiv c1 c3.
+
+  unfold cequiv.
+  split; intros.
+  apply H0. apply H; auto.
+  apply H. apply H0 ;auto.
+Qed.
+
+
+Theorem CAss_congruence :
+  forall i a1 a1',
+    aequiv a1 a1' ->
+    cequiv (CAss i a1) (CAss i a1').
+  split; intros.
+  inversion H0. apply E_Ass. pose (H st). rewrite <- e. auto.
+  inversion H0. apply E_Ass. pose (H st). rewrite e. auto.
+Qed.
+
+Theorem CWhile_congruence:
+  forall b1 b1' c1 c1',
+         bequiv b1 b1' ->
+         cequiv c1 c1' ->
+         cequiv (WHILE b1 DO c1 END)
+                (WHILE b1' DO c1' END).
+
+  split; intros. generalize dependent b1'. generalize dependent c1'.
+  remember (WHILE b1 DO c1 END) as h1. generalize dependent Heqh1.
+  elim H1; try (simpl; intros; discriminate).
+  intros. pose (H4 Heqh1 c1' H5 b1' H6).
+  eapply E_WhileLoop. inversion Heqh1. pose (H6 st0). rewrite <- e. rewrite <- H8. auto.
+  inversion Heqh1. apply H5. rewrite <- H9. apply H0. apply c0.
+  intros. pose (H2 st0). inversion Heqh1. subst b1. rewrite H in e. apply E_WhileEnd. auto.
+  generalize dependent b1. generalize dependent c1.
+  remember (WHILE b1' DO c1' END) as h1.
+  generalize Heqh1. elim H1; try (simpl; intros; discriminate).
+  intros. inversion Heqh0. pose (H4 Heqh0 c1 H5 b1 H6).
+  eapply E_WhileLoop. rewrite H6. rewrite <- H8. auto.
+  apply H5. rewrite <- H9. apply H0. auto.
+  intros. apply E_WhileEnd. rewrite H2. inversion Heqh0. subst b1'. auto.
+Qed.
+
+Theorem CSeq_congruence :
+  forall c1 c1' c2 c2',
+    cequiv c1 c1' ->
+    cequiv c2 c2' ->
+    cequiv (c1;;c2) (c1';;c2).
+  split.
+  intros. inversion H1. eapply E_Seq. apply H. apply H4. apply H7.
+  intros. inversion H1. eapply E_Seq. apply H. apply H4. apply H7.
+Qed.
+
+
+Theorem CIf_congruence:
+  forall b b' c1 c1' c2 c2',
+    bequiv b b' ->
+    cequiv c1 c1' ->
+    cequiv c2 c2' ->
+    cequiv (IFB b THEN c1 ELSE c2 FI)
+           (IFB b' THEN c1' ELSE c2' FI).
+  split; intros.
+  inversion H2. apply E_IfTrue. pose (H st). rewrite <- e. auto.
+  apply H0. auto.
+  apply E_IfFalse. rewrite <- H. auto.
+  apply H1. auto.
+  inversion H2. apply E_IfTrue. rewrite H. auto. apply H0. auto.
+  apply E_IfFalse. rewrite H. auto. apply H1. auto.
+Qed.
+
+Definition atrans_sound (atrans: aexp -> aexp) : Prop :=
+  forall (a:aexp),
+    aequiv a (atrans a).
+
+Definition btrans_sound (btrans: bexp -> bexp) : Prop :=
+  forall (b:bexp),
+    bequiv b (btrans b).
+
+Definition ctrans_sound (ctrans : com -> com) : Prop :=
+  forall (c : com),
+    cequiv c (ctrans c).
+
+Fixpoint fold_constants_aexp (a:aexp) : aexp :=
+  match a with
+    | ANum n => ANum n
+    | AId i => AId i
+    | APlus a1 a2 =>
+      match (fold_constants_aexp a1, fold_constants_aexp a2)
+      with
+        | (ANum n1, ANum n2) => ANum (n1 + n2)
+        | (a1' , a2') => APlus a1' a2'
+      end
+    | AMinus a1 a2 =>
+      match (fold_constants_aexp a1, fold_constants_aexp a2) with
+        | (ANum n1, ANum n2) => ANum (n1 - n2)
+        | (a1', a2') => AMinus a1' a2'
+      end
+    | AMult a1 a2 =>
+      match (fold_constants_aexp a1, fold_constants_aexp a2) with
+        | (ANum n1, ANum n2) => ANum (n1 * n2)
+        | (a1', a2') => AMult a1' a2'
+      end
+  end.
+
+Example fold_aexp_ex1 :
+  fold_constants_aexp (AMult (APlus (ANum 1) (ANum 2)) (AId X))
+  = AMult (ANum 3) (AId X).
+simpl; auto.
+Qed.
+
+Print eq_nat_dec.
+SearchPattern ({_}+{_}).
+
+Fixpoint fold_constants_bexp (b:bexp) : bexp :=
+  match b with
+    | BTrue => BTrue
+    | BFalse => BFalse
+    | BEq a1 a2 =>
+      match (fold_constants_aexp a1, fold_constants_aexp a2) with
+        | (ANum n1, ANum n2) =>
+          if (eq_nat_dec n1 n2) then BTrue else BFalse
+        | (a1', a2') => BEq a1' a2'
+      end
+    | BLe a1 a2 =>
+      match (fold_constants_aexp a1, fold_constants_aexp a2) with
+        | (ANum n1, ANum n2) =>
+          if (le_dec n1 n2) then BTrue else BFalse
+        | (a1' ,a2') => BLe a1' a2'
+      end
+    | BNot b1 =>
+      match (fold_constants_bexp b1) with
+        | BTrue => BFalse
+        | BFalse => BTrue
+        | b1' => BNot b1'
+      end
+    | BAnd b1 b2 =>
+      match (fold_constants_bexp b1, fold_constants_bexp b2) with
+        | (BTrue, BFalse) => BFalse
+        | (BTrue, BTrue) => BTrue
+        | (BFalse, BTrue) => BFalse
+        | (BFalse, BFalse) => BFalse
+        | (b1', b2') => BAnd b1' b2'
+      end
+  end.
+
+Fixpoint fold_constants_com (c:com) : com :=
+  match c with
+    | SKIP => SKIP
+    | i ::= a => CAss i (fold_constants_aexp a)
+    | c1 ;; c2 => (fold_constants_com c1);;(fold_constants_com c2)
+    | IFB b THEN c1 ELSE c2 FI =>
+      match fold_constants_bexp b with
+        | BTrue => fold_constants_com c1
+        | BFalse => fold_constants_com c2
+        | b' => IFB b' THEN (fold_constants_com c1) ELSE (fold_constants_com c2) FI
+      end
+    | WHILE b DO c END =>
+      match fold_constants_bexp b with
+        | BTrue => WHILE BTrue DO SKIP END
+        | BFalse => SKIP
+        | b' => WHILE b' DO (fold_constants_com c) END
+      end
+  end.
+
+
+
+
+Lemma fca_plus:
+  forall a1 a2 st,
+    aeval st (fold_constants_aexp (APlus a1 a2)) =
+    aeval st (APlus (fold_constants_aexp a1) (fold_constants_aexp a2)).
+  simpl. intros a1 a2. destruct (fold_constants_aexp a1) eqn: h1; destruct (fold_constants_aexp a2); try(simpl; auto; fail).
+Qed.
+
+
+
+Lemma fca_minus:
+  forall a1 a2 st,
+    aeval st (fold_constants_aexp (AMinus a1 a2)) =
+    aeval st (AMinus (fold_constants_aexp a1) (fold_constants_aexp a2)).
+  simpl. intros a1 a2. destruct (fold_constants_aexp a1) eqn: h1; destruct (fold_constants_aexp a2); try(simpl; auto; fail).
+Qed.
+
+Lemma fca_mult:
+  forall a1 a2 st,
+    aeval st (fold_constants_aexp (AMult a1 a2)) =
+    aeval st (AMult (fold_constants_aexp a1) (fold_constants_aexp a2)).
+  simpl. intros a1 a2. destruct (fold_constants_aexp a1) eqn: h1; destruct (fold_constants_aexp a2); try(simpl; auto; fail).
+Qed.
+
+
+
+
+Lemma aexp_plus_aplus:
+  forall a1 a2 st,
+    aeval st (APlus a1 a2) = aeval st a1 + aeval st a2.
+  auto.
+Qed.
+
+Lemma aexp_minus_aminus:
+  forall a1 a2 st,
+    aeval st (AMinus a1 a2) = aeval st a1 - aeval st a2.
+  auto.
+Qed.
+
+Lemma aexp_mult_amult:
+  forall a1 a2 st,
+    aeval st (AMult a1 a2) = aeval st a1 * aeval st a2.
+  auto.
+Qed.
+
+Hint Rewrite aexp_plus_aplus aexp_minus_aminus aexp_mult_amult fca_plus fca_mult fca_minus : fca_rwbase.
+
+Theorem fold_constants_aexp_sound :
+  atrans_sound fold_constants_aexp.
+  unfold atrans_sound.
+  unfold aequiv.
+  intro. elim a; try (auto); try (intros; autorewrite with fca_rwbase);rewrite H; rewrite H0; autorewrite with fca_rwbase; auto.
+Qed.
+
+
+
+Theorem fold_constants_bexp_sound :
+  btrans_sound fold_constants_bexp.
+  unfold btrans_sound. unfold bequiv.
+  intro. elim b; try (simpl; auto; fail);
+         try (intros; simpl; rewrite (fold_constants_aexp_sound a); rewrite (fold_constants_aexp_sound a0); destruct (fold_constants_aexp a); destruct (fold_constants_aexp a0); try (simpl; auto; fail));
+         try (intros; simpl; try (rewrite H); try (rewrite H0); try (rewrite H1); destruct (fold_constants_bexp b0); try (destruct (fold_constants_bexp b1)); try (simpl; auto; fail); fail).
+  unfold beq_nat_bydec; intros; simpl; case (eq_nat_dec n n0); simpl; auto.
+  unfold leb_bydec; intros; simpl; case (le_dec n n0); simpl; auto.
+Qed.
+
+
+
+Theorem fold_constants_com_sound:
+  ctrans_sound fold_constants_com.
+
+  unfold ctrans_sound. unfold cequiv.
+  intro. split; generalize dependent st; generalize dependent st'.
+  elim c; try (simpl; auto; fail); intros.
+  simpl. inversion H. rewrite (fold_constants_aexp_sound a) in H4. rewrite <- H4.
+  apply E_Ass; auto.
+  simpl. inversion H1. pose (H _ _ H4). pose (H0 _ _ H7). eapply E_Seq. apply c4. apply c5.
+  inversion H1. pose (H _ _ H8). pose (fold_constants_bexp_sound b st).
+  rewrite H7 in e; symmetry in e.
+  simpl; destruct (fold_constants_bexp b) eqn:hh ; try (simpl; auto; fail);
+  try (rewrite H7 in hh; discriminate); try (rewrite e; simpl; auto); try (simpl in e; discriminate); try (apply E_IfTrue; auto).
+  pose (H0 _ _ H8). pose (fold_constants_bexp_sound b st).
+  rewrite H7 in e; symmetry in e.
+ simpl; destruct (fold_constants_bexp b) eqn:hh ; try (simpl; auto; fail);
+ try (rewrite H7 in hh; discriminate); try (rewrite e; simpl; auto); try (simpl in e; discriminate); try (apply E_IfFalse; auto).
+ clear c. remember (WHILE b DO c0 END) as h. generalize dependent Heqh. elim H0; try (simpl; intros; discriminate).
+ intros. inversion Heqh; subst b0; subst c0.
+ destruct (fold_constants_bexp b) eqn: hh;
+   pose (H5 eq_refl) as h2;
+   simpl; simpl in h2; rewrite hh in h2; rewrite hh; pose (E_WhileLoop b c st0 st'0 st'' H1 H2 H4) as h0; (try auto).
+ apply (WHILE_true b c). pose (fold_constants_bexp_sound b). rewrite hh in b0. auto.
+ auto. pose (fold_constants_bexp_sound b st0) as h'; rewrite H1 in h'; rewrite hh in h'; simpl in h'; discriminate.
+ eapply E_WhileLoop. rewrite <- hh. rewrite <- fold_constants_bexp_sound. auto. apply H. apply H2; auto. auto.
+ eapply E_WhileLoop. rewrite <- hh. rewrite <- fold_constants_bexp_sound. auto. apply H. apply H2; auto. auto.
+ eapply E_WhileLoop. rewrite <- hh. rewrite <- fold_constants_bexp_sound. auto. apply H. apply H2; auto. auto. 
+ eapply E_WhileLoop. rewrite <- hh. rewrite <- fold_constants_bexp_sound. auto. apply H. apply H2; auto. auto.
+ intros. inversion Heqh; subst b0; subst c0.
+ simpl; destruct (fold_constants_bexp b) eqn:hh; pose (fold_constants_bexp_sound b st0) as h1; rewrite H1 in h1; rewrite hh in h1; simpl in h1; (try discriminate); try ( apply E_WhileEnd; simpl; rewrite h1; auto).
+ apply E_Skip.
+ elim c; try auto.
+ intros. pose (CAss_congruence i a (fold_constants_aexp a) (fold_constants_aexp_sound a) st st').
+ destruct i0. auto.
+ intros. inversion H1. Print E_Seq. apply (E_Seq _ _ st st'0); auto.
+ intros. simpl in H1; destruct (fold_constants_bexp b) eqn:hh;
+         try( apply E_IfTrue; pose (fold_constants_bexp_sound b st) as e; rewrite hh in e; try( rewrite e; auto); auto; fail);
+         try( apply E_IfFalse; pose (fold_constants_bexp_sound b st) as e; rewrite hh in e; try( rewrite e; auto); auto; fail).
+ inversion H1; [apply E_IfTrue | apply E_IfFalse]; pose (fold_constants_bexp_sound b st) as h3; rewrite hh in  h3; try( try rewrite h3; auto; apply H; auto; fail); try ( try rewrite h3; auto; apply H0; auto; fail).
+ inversion H1; [apply E_IfTrue | apply E_IfFalse]; pose (fold_constants_bexp_sound b st) as h3; rewrite hh in  h3; try( try rewrite h3; auto; apply H; auto; fail); try ( try rewrite h3; auto; apply H0; auto; fail).
+ inversion H1; [apply E_IfTrue | apply E_IfFalse]; pose (fold_constants_bexp_sound b st) as h3; rewrite hh in  h3; try( try rewrite h3; auto; apply H; auto; fail); try ( try rewrite h3; auto; apply H0; auto; fail).
+ inversion H1; [apply E_IfTrue | apply E_IfFalse]; pose (fold_constants_bexp_sound b st) as h3; rewrite hh in  h3; try( try rewrite h3; auto; apply H; auto; fail); try ( try rewrite h3; auto; apply H0; auto; fail).
+ intros. simpl in H0. destruct (fold_constants_bexp b) eqn:hh.
+ apply (WHILE_true b c0). pose (fold_constants_bexp_sound b). rewrite hh in b0; auto. auto.
+ inversion H0. apply E_WhileEnd. pose (fold_constants_bexp_sound b st'). rewrite hh in e; rewrite e; auto.
+ rewrite <- hh in H0.
+ remember (WHILE fold_constants_bexp b DO fold_constants_com c0 END) as h. generalize dependent Heqh. elim H0; try(simpl; intros; discriminate).
+ intros. inversion Heqh; subst b0; subst c1. pose (H st'0 st0 H2). pose (H5 eq_refl). eapply E_WhileLoop. rewrite fold_constants_bexp_sound. auto. apply c1. apply c2.
+ intros. inversion Heqh; subst b0 ; subst c1. apply E_WhileEnd. rewrite fold_constants_bexp_sound. auto.
+ rewrite <- hh in H0.
+ remember (WHILE fold_constants_bexp b DO fold_constants_com c0 END) as h. generalize dependent Heqh. elim H0; try(simpl; intros; discriminate).
+ intros. inversion Heqh; subst b0; subst c1. pose (H st'0 st0 H2). pose (H5 eq_refl). eapply E_WhileLoop. rewrite fold_constants_bexp_sound. auto. apply c1. apply c2.
+ intros. inversion Heqh; subst b0 ; subst c1. apply E_WhileEnd. rewrite fold_constants_bexp_sound. auto.
+ rewrite <- hh in H0.
+ remember (WHILE fold_constants_bexp b DO fold_constants_com c0 END) as h. generalize dependent Heqh. elim H0; try(simpl; intros; discriminate).
+ intros. inversion Heqh; subst b1; subst c1. pose (H st'0 st0 H2). pose (H5 eq_refl). eapply E_WhileLoop. rewrite fold_constants_bexp_sound. auto. apply c1. apply c2.
+ intros. inversion Heqh; subst b1 ; subst c1. apply E_WhileEnd. rewrite fold_constants_bexp_sound. auto.
+ rewrite <- hh in H0.
+ remember (WHILE fold_constants_bexp b DO fold_constants_com c0 END) as h. generalize dependent Heqh. elim H0; try(simpl; intros; discriminate).
+ intros. inversion Heqh; subst b0; subst c1. pose (H st'0 st0 H2). pose (H5 eq_refl). eapply E_WhileLoop. rewrite fold_constants_bexp_sound. auto. apply c1. apply c2.
+ intros. inversion Heqh; subst b0 ; subst c1. apply E_WhileEnd. rewrite fold_constants_bexp_sound. auto.
+Qed.
+
+Theorem inequiv_exercise:
+  ~ cequiv (WHILE BTrue DO SKIP END)
+    SKIP.
+
+  unfold not; unfold cequiv. intros.
+  pose (E_Skip (t_empty 0)).
+  pose (H (t_empty 0) (t_empty 0)).
+  destruct i. pose (H1 c).
+  SearchPattern ( _ / _ \\ _).
+  pose loop_never_stops.
+  pose (n loop (t_empty 0) (t_empty 0) eq_refl). unfold loop in n0.
+  unfold not in n0. auto.
+Qed.
+
+Module HIMP.
+
+  Inductive com : Type :=
+| CSkip : com
+| CAss : id -> aexp -> com
+| CSeq : com -> com -> com
+| CIf : bexp -> com -> com -> com
+| CWhile : bexp -> com -> com
+| CHavoc : id -> com.
+
+  Notation "'SKIP'" :=
+    CSkip.
+
+  Notation "X '::=' a":=
+    (CAss X a) (at level 60).
+
+  Notation "c1 ;; c2" :=
+    (CSeq c1 c2) (at level 80, right associativity).
+
+  Notation "'WHILE' b 'DO' c 'END'" :=
+    (CWhile b c) (at level 80, right associativity).
+
+  Notation "'IFB' b 'THEN' c1 'ELSE' c2 'END'" :=
+    (CIf b c1 c2) (at level 80, right associativity).
+
+  Notation "'HAVOC' l" := (CHavoc l) (at level 60).
+
+  Reserved Notation "c1 '/' st '\\' st'"
+           (at level 40, st at level 39).
+
+
+End HIMP.
+
+
